src/mappers/abstractFunction.ts
@@ -2,13 +2,13 @@ import { TSESTree } from "@typescript-eslint/typescript-estree";
 import AbstractMapper, { MapContext, MapOptions } from "./abstract";
 import BlockStatementMapper from "./blockStatement";
 import { Dafny } from "../types";
-import { createBoolType_, createClassMemberDecl, createDomainType_, createFormals, createGIndentType, createIndentType, createMethodDecl, createStringType_, createType } from "../typeCreate";
+import { createBoolType_, createClassMemberDecl, createDomainType_, createFormals, createFunctionBody, createFunctionDecl, createFunctionSignature_, createGIndentType, createIndentType, createMethodDecl, createPredicateSignature_, createStringType_, createType } from "../typeCreate";
 
 abstract class AbstractFunctionMapper<T extends TSESTree.FunctionDeclaration|TSESTree.FunctionExpression> extends AbstractMapper<T,Dafny.ClassMemberDecl> {
 	id?: TSESTree.Identifier;
 
 	constructor(node: T, options: MapOptions, context: MapContext, id?: TSESTree.Identifier) {
-		context.methodSpec = [];
+		context.spec = [];
 		context.types = context.types.getCopy();
 		super(node, options, context);
 		this.id = id;
@@ -31,7 +31,29 @@ abstract class AbstractFunctionMapper<T extends TSESTree.FunctionDeclaration|TSE
 			}
 		}
 
-		return createClassMemberDecl(createMethodDecl(id.name, "method", value, createFormals(parameters), createFormals(returns), this.context.methodSpec));
+		if (value.value.length === 1 && value.value[0].value.type === "ReturnStmt") {
+			const body = createFunctionBody(value.value[0].value.value[0].value);
+
+			if(returns[0].value.type_.value.value.value === "bool") {
+				return createClassMemberDecl(createFunctionDecl(
+					id.name, 
+					body, 
+					createPredicateSignature_(createFormals(parameters)), 
+					this.context.spec
+				));
+			}
+			else {
+				return createClassMemberDecl(createFunctionDecl(
+					id.name, 
+					body, 
+					createFunctionSignature_(createFormals(parameters), returns[0].value.type_), 
+					this.context.spec
+				));
+			}
+		}
+		else {
+			return createClassMemberDecl(createMethodDecl(id.name, "method", value, createFormals(parameters), createFormals(returns), this.context.spec));
+		}
 	}
 
 	returnType(): Dafny.Type|undefined {
